test/assumptions.t
@@ -1,19 +1,5 @@
   $ rocq compile -q -noglob -R ../src FMV -o assumptions.vo assumptions.v
   Axioms:
   Impl.sat is assumed to be guarded.
-  backtrack_progress_falsified_pending :
-    forall (s : Impl.State) (cause : Impl.Clause) (next : Impl.State),
-    backtrack_invariant s ->
-    clause_implied_by_store (Impl.state_clauses s) cause ->
-    clause_falsified_by_model (Impl.trail_model (Impl.state_trail s)) cause ->
-    Impl.backtrack (s, cause) = Some (Impl.Progress next) ->
-    falsified_clauses_pending next
   Axioms:
   Impl.sat is assumed to be guarded.
-  backtrack_progress_falsified_pending :
-    forall (s : Impl.State) (cause : Impl.Clause) (next : Impl.State),
-    backtrack_invariant s ->
-    clause_implied_by_store (Impl.state_clauses s) cause ->
-    clause_falsified_by_model (Impl.trail_model (Impl.state_trail s)) cause ->
-    Impl.backtrack (s, cause) = Some (Impl.Progress next) ->
-    falsified_clauses_pending next
